removed existential quantification and implemented many assumptions found a logical bug

lib/smem/st3.fst
@@ -1,13 +1,14 @@
 (*--build-config
     options:--admit_fsi Set;
     variables:LIB=..;
-    other-files:$LIB/ext.fst $LIB/set.fsi $LIB/heap.fst $LIB/st.fst stack.fst $LIB/list.fst
+    other-files:$LIB/ext.fst $LIB/set.fsi $LIB/heap.fst $LIB/st.fst $LIB/list.fst stack.fst
   --*)
 
 module StructuredMem
 open Heap
 open Stack
 open Set
+open Prims
 
 type sidt = nat
 
@@ -20,8 +21,21 @@ type smem = heap * memStack
 
 (*rename heap to memblock, and then hp to heap*)
 let hp (s : smem) = fst s
+
+val st : smem -> Tot (Stack (sidt * heap))
 let st (s : smem) = fst (snd s)
+
 let sid (s : (sidt * heap)) = fst s
+
+val topst : (s:smem{ (snonempty (st s)) == true}) -> Tot  (sidt * heap)
+let topst ss = (top (st ss))
+
+val topstb : (s:smem{ (snonempty (st s)) == true}) ->  Tot heap
+let topstb ss = snd (topst ss)
+
+val topstid : (s:smem{ (snonempty (st s)) == true}) ->  Tot sidt
+let topstid ss = fst (topst ss)
+
 
 new_effect StSTATE = STATE_h smem
 
@@ -45,29 +59,74 @@ assume val refLoc : #a:Type -> ref a -> Tot refLocType
 assume val blockAtLoc : smem -> refLocType  -> Tot (option heap)
 
 
-type allocateInBlock (#a:Type) (r: ref a) (h0 : heap) (h1 : heap) (init : a)   = not(contains h0 r) /\ contains h1 r /\  h1 == upd h1 r init
+type allocateInBlock (#a:Type) (r: ref a) (h0 : heap) (h1 : heap) (init : a)   = not(contains h0 r) /\ contains h1 r /\  h1 == upd h0 r init
 
 
 
-assume val alloc:  #a:Type -> init:a -> ST (ref a)
+assume val halloc:  #a:Type -> init:a -> ST (ref a)
                                          (fun m -> True)
                                          (fun m0 r m1 -> allocateInBlock r (hp m0)  (hp m1) init /\ (st m0 == st m1) /\ refLoc r == InHeap)
 
-
 assume val salloc:  #a:Type -> init:a -> ST (ref a)
-                                         (fun m -> True)
-                                         (fun m0 r m1 -> exists s0. exists s1. (isTop s0 (st m0)) /\ (isTop s1 (st m1)) /\ allocateInBlock r (snd s0)  (snd s1) init
-                                         		/\ refLoc r == InStack (sid s0) /\ sid s0 = sid s1 /\ btail (st m0) == btail (st m1) /\ (hp m0) == hp m1)
+     (fun m -> (snonempty (st m) == true))
+     (fun m0 r m1 ->
+          (snonempty (st m0) == true) /\ (snonempty (st m1)) == true
+          /\ allocateInBlock r (topstb m0) (topstb m0) init
+          /\ refLoc r == InStack (topstid m0) /\ (topstid m0 = topstid m1)
+          /\ stail (st m0) == stail (st m1) /\ (hp m0) == hp m1)
+
+(*HELP : how to write this:
+val refExistsInMem : #a:Type -> (ref a) -> smem ->  Tot Type
+let refExistsInMem (#a:Type) (r:ref a) (m:smem) =
+match (blockAtLoc m (refLoc r)) with
+          | Some b -> contains b r
+          | None -> false
+*)
+
+val refExistsInMem : #a:Type -> (ref a) -> smem ->  Tot bool
+let refExistsInMem (#a:Type) (r:ref a) (m:smem) =
+match (blockAtLoc m (refLoc r)) with
+          | Some b -> contains b r
+          | None -> false
+
+(* BUG: sel should not always return something, it would be tricky to implement it.
+  what prevents me from creating a ref of an empty type?
+*)
+val loopkupRef : #a:Type -> (ref a) -> smem ->  Tot (option a)
+let loopkupRef (#a:Type) (r:ref a) (m:smem) =
+match (blockAtLoc m (refLoc r)) with
+          | Some b -> Some (sel b r)
+          | None -> None
 
 assume val read:  #a:Type -> r:(ref a) -> ST a
-                                      	    (fun m -> exists b. blockAtLoc m (refLoc r) = Some b /\ contains b r)
-                                            (fun m0 a m1 -> exists b. m0=m1 /\ blockAtLoc m0 (refLoc r) = Some b /\ sel b r == a)
+	  (fun m -> (refExistsInMem r m) == true)
+    (fun m0 a m1 -> m0=m1 /\ loopkupRef r m0 = Some a)
 
-(**
-open List
-let sids (m : smem) = map fst (st m)
 
-type notIn  (#a:Type) (e : a) (l : list a) : Tot Type  = a
+val lmap : #a:Type -> #b:Type -> (a -> Tot b) -> (list a) -> Tot (list b)
+let rec lmap f l =
+match l with
+| nil -> []
+| h::tl -> (f h)::(lmap f tl)
+
+
+val sids : smem -> Tot (list sidt)
+let sids (m : smem) = lmap fst (st m)
+
+assume val inList : sidt -> (list sidt) -> Tot bool
+
+assume val newStackFrame:  unit -> ST unit
+    (fun m -> True)
+    (fun m0 a m1 -> stail (st m1) = (st m0) /\ (snonempty (st m1) == true) /\ ((inList (topstid m1) (sids m0)) == false) /\ (topstb m1) = emp)
+
+
+(*
+assume val write:  #a:Type -> r:(ref a) -> ST unit
+	    (fun m -> (refExistsInMem r m) == true)
+      (fun m0 a m1 -> m0=m1 /\ loopkupRef r m0 = Some a)
+*)
+
+(*
 
 
 assume val newStackFrame:  unit -> ST unit
